sf/Assignment08_01.v
@@ -7,11 +7,15 @@ Example ceval_example2:
     (X ::= ANum 0;; Y ::= ANum 1;; Z ::= ANum 2) / empty_state ||
     (update (update (update empty_state X 0) Y 1) Z 2).
 Proof.
-  exact FILL_IN_HERE.
+  apply E_Seq with (update empty_state X 0).
+  - apply E_Ass. reflexivity.
+  - apply E_Seq with (update (update empty_state X 0) Y 1).
+    + apply E_Ass. reflexivity.
+    + apply E_Ass. reflexivity.
 Qed.
 
 (*-- Check --*)
-Check ceval_example2 : 
+Check ceval_example2 :
     (X ::= ANum 0;; Y ::= ANum 1;; Z ::= ANum 2) / empty_state ||
     (update (update (update empty_state X 0) Y 1) Z 2).
 
