sf/Assignment08_02.v
@@ -9,14 +9,31 @@ Require Export Assignment08_01.
    (this latter part is trickier than you might expect). *)
 
 Definition pup_to_n : com :=
-  FILL_IN_HERE.
+  Y ::= ANum 0;;
+  WHILE BNot (BEq (AId X) (ANum 0)) DO
+    Y ::= APlus (AId X) (AId Y);;
+    X ::= AMinus (AId X) (ANum 1)
+  END.
 
 Example pup_to_2_ceval :
   pup_to_n / (update empty_state X 2) ||
     update (update (update (update (update (update empty_state
       X 2) Y 0) Y 2) X 1) Y 3) X 0.
 Proof.
-  exact FILL_IN_HERE.
+  apply E_Seq with (update (update empty_state X 2) Y 0).
+  - apply E_Ass. reflexivity.
+  - apply E_WhileLoop with (update (update (update (update empty_state X 2) Y 0) Y 2) X 1).
+    + auto.
+    + apply E_Seq with (update (update (update empty_state X 2) Y 0) Y 2).
+      * apply E_Ass. reflexivity.
+      * apply E_Ass. reflexivity.
+    + apply E_WhileLoop with (update (update (update (update (update (update empty_state X 2) Y 0) Y 2) X 1) Y 3) X 0).
+      * auto.
+      * apply E_Seq with (update (update (update (update (update empty_state X 2) Y 0) Y 2) X 1) Y 3).
+        { apply E_Ass. reflexivity. }
+        { apply E_Ass. reflexivity. }
+      * apply E_WhileEnd. reflexivity.
+
 Qed.
 
 (*-- Check --*)
@@ -24,4 +41,4 @@ Check pup_to_2_ceval :
   pup_to_n / (update empty_state X 2) ||
     update (update (update (update (update (update empty_state
       X 2) Y 0) Y 2) X 1) Y 3) X 0.
- 
+
