sf/Assignment08_03.v
@@ -8,11 +8,14 @@ Theorem loop_never_stops : forall st st',
 Proof.
   intros st st' contra. unfold loop in contra.
   remember (WHILE BTrue DO SKIP END) as loopdef eqn:Heqloopdef.
-    (* Proceed by induction on the assumed derivation showing that
-     [loopdef] terminates.  Most of the cases are immediately
-     contradictory (and so can be solved in one step with
-     [inversion]). *)
-  exact FILL_IN_HERE.
+  induction contra.
+  - inversion Heqloopdef.
+  - inversion Heqloopdef.
+  - inversion Heqloopdef.
+  - inversion Heqloopdef.
+  - inversion Heqloopdef.
+  - inversion Heqloopdef. subst. inversion H.
+  - apply IHcontra2. apply Heqloopdef.
 Qed.
 
 (*-- Check --*)
