sf/Assignment08_04.v
@@ -13,7 +13,20 @@ Theorem no_whiles_terminate: forall c st
     (NOWHL: no_whiles c = true),
   exists st', c / st || st'.
 Proof.
-  exact FILL_IN_HERE.
+  intros. generalize dependent st. induction c.
+  - intros. exists st. apply E_Skip.
+  - intros. exists (update st i (aeval st a)). apply E_Ass. reflexivity.
+  - intros. inversion NOWHL. apply andb_true_iff in H0. destruct H0.
+    assert (exists st', c1 / st || st'). apply IHc1. apply H.
+    inversion H1.
+    assert (exists st'', c2 / x|| st''). apply IHc2. apply H0.
+    inversion H3. exists x0. apply E_Seq with x. apply H2. apply H4.
+  - intros. inversion NOWHL. apply andb_true_iff in H0. destruct H0.
+    assert (exists st', c1 / st || st'). apply IHc1. apply H.
+    inversion H1.
+    assert (exists st'', c2 / st|| st''). apply IHc2. apply H0.
+    inversion H3. destruct (beval st b) eqn:AA. exists x. apply E_IfTrue. apply AA. apply H2. exists x0. apply E_IfFalse. apply AA. apply H4.
+  - intros. inversion NOWHL.
 Qed.
 
 (*-- Check --*)
