sf/Assignment08_06.v
@@ -7,16 +7,18 @@ Require Export Assignment08_05.
     program *)
 
 Theorem skip_right: forall c,
-  cequiv 
-    (c;; SKIP) 
+  cequiv
+    (c;; SKIP)
     c.
-Proof. 
-  exact FILL_IN_HERE.
+Proof.
+  intros c st st'.
+  split. intros. inversion H. subst. inversion H5. subst. apply H2.
+  intros. apply E_Seq with st'. apply H. apply E_Skip.
 Qed.
 
 (*-- Check --*)
 Check skip_right: forall c,
-  cequiv 
-    (c;; SKIP) 
+  cequiv
+    (c;; SKIP)
     c.
 
