sf/Assignment08_07.v
@@ -5,17 +5,20 @@ Require Export Assignment08_06.
 (** **** Exercise: 2 stars (IFB_false)  *)
 Theorem IFB_false: forall b c1 c2,
   bequiv b BFalse  ->
-  cequiv 
-    (IFB b THEN c1 ELSE c2 FI) 
+  cequiv
+    (IFB b THEN c1 ELSE c2 FI)
     c2.
 Proof.
-  exact FILL_IN_HERE.
+  intros.
+  intros st st'.
+  split. intros. inversion H0. subst. unfold bequiv in H. rewrite H in H6. inversion H6. subst. apply H7.
+  intros. apply E_IfFalse. unfold bequiv in H. rewrite H. simpl. reflexivity. apply H0.
 Qed.
 
 (*-- Check --*)
 Check IFB_false: forall b c1 c2,
   bequiv b BFalse  ->
-  cequiv 
-    (IFB b THEN c1 ELSE c2 FI) 
+  cequiv
+    (IFB b THEN c1 ELSE c2 FI)
     c2.
 
