sf/Assignment08_08.v
@@ -11,7 +11,13 @@ Theorem swap_if_branches: forall b e1 e2,
     (IFB b THEN e1 ELSE e2 FI)
     (IFB BNot b THEN e2 ELSE e1 FI).
 Proof.
-  exact FILL_IN_HERE.
+  intros.
+  intros st st'.
+  split. intros.
+  inversion H. subst. apply E_IfFalse. simpl. rewrite H5. reflexivity. apply H6.
+  subst. apply E_IfTrue. simpl. rewrite H5. reflexivity. apply H6.
+  intros. inversion H. subst. simpl in H5. apply E_IfFalse. apply negb_true_iff in H5. apply H5. apply H6.
+  subst. simpl in H5. apply negb_false_iff in H5. apply E_IfTrue. apply H5. apply H6.
 Qed.
 
 (*-- Check --*)
