sf/Assignment08_10.v
@@ -6,7 +6,10 @@ Require Export Assignment08_09.
 Theorem seq_assoc : forall c1 c2 c3,
   cequiv ((c1;;c2);;c3) (c1;;(c2;;c3)).
 Proof.
-  exact FILL_IN_HERE.
+  intros. unfold cequiv.
+  split. intros.
+  inversion H. subst. inversion H2. subst. apply E_Seq with st'1. apply H3. apply E_Seq with st'0. apply H7. apply H5.
+  intros. inversion H. subst. inversion H5. subst. apply E_Seq with st'1. apply E_Seq with st'0. apply H2. apply H3. apply H7.
 Qed.
 
 (*-- Check --*)
