sf/Assignment08_11.v
@@ -2,16 +2,24 @@ Require Export Assignment08_10.
 
 (* problem #11: 10 points *)
 
+Theorem update_same : forall n1 x1 x2 (st : state),
+  st x1 = n1 ->
+  (update st x1 n1) x2 = st x2.
+Proof.
+  intros. unfold update. destruct (eq_id_dec x1 x2). rewrite <- e. rewrite H. reflexivity.
+  reflexivity.
+Qed.
+
 (** **** Exercise: 2 stars (assign_aequiv)  *)
 Theorem assign_aequiv : forall X e,
-  aequiv (AId X) e -> 
+  aequiv (AId X) e ->
   cequiv SKIP (X ::= e).
 Proof.
-  exact FILL_IN_HERE.
+  intros. intros st st'. split; intros. inversion H0; subst. assert(HH: st' = (update st' X (st' X))). apply functional_extensionality. intros. rewrite update_same. reflexivity. reflexivity. rewrite HH at 2. constructor. unfold aequiv in H. rewrite <- H. simpl. reflexivity. inversion H0. subst. replace (update st X (aeval st e)) with st. constructor. unfold aequiv in H. rewrite <- H. simpl. apply functional_extensionality. intros. rewrite update_same. reflexivity. reflexivity.
 Qed.
 
 (*-- Check --*)
 Check assign_aequiv : forall X e,
-  aequiv (AId X) e -> 
+  aequiv (AId X) e ->
   cequiv SKIP (X ::= e).
 
