sf/Assignment08_13.v
@@ -7,7 +7,12 @@ Theorem CIf_congruence : forall b b' c1 c1' c2 c2',
   bequiv b b' -> cequiv c1 c1' -> cequiv c2 c2' ->
   cequiv (IFB b THEN c1 ELSE c2 FI) (IFB b' THEN c1' ELSE c2' FI).
 Proof.
-  exact FILL_IN_HERE.
+  intros. intros st st'. split. intros. inversion H2; subst.
+  apply E_IfTrue. unfold bequiv in H. rewrite <- H. apply H8. apply H0. apply H9.
+  apply E_IfFalse. unfold bequiv in H. rewrite <- H. apply H8. apply H1. apply H9.
+  intros. inversion H2; subst.
+  apply E_IfTrue. unfold bequiv in H. rewrite H. apply H8. apply H0. apply H9.
+  apply E_IfFalse. unfold bequiv in H. rewrite H. apply H8. apply H1. apply H9.
 Qed.
 
 (*-- Check --*)
