sf/Assignment08_16.v
@@ -5,7 +5,30 @@ Require Export Assignment08_15.
 Lemma optimize_0plus_aexp_sound:
   atrans_sound optimize_0plus_aexp.
 Proof.
-  exact FILL_IN_HERE.
+
+  unfold atrans_sound. intros. unfold aequiv. intros. induction a; try constructor; try( simpl; rewrite IHa1; rewrite IHa2; reflexivity).
+  simpl. destruct a1.
+  destruct a2;
+    try destruct n; try destruct n0; simpl; try omega;
+    try(simpl in IHa2; rewrite IHa2; reflexivity).
+  destruct a2;
+    try destruct n; try destruct n0; simpl; try omega;
+    try(simpl in IHa2; rewrite IHa2; reflexivity).
+  destruct a2;
+    try (rewrite IHa1; rewrite IHa2; simpl; reflexivity);
+    destruct n;
+      try(rewrite IHa1; reflexivity);
+      try( rewrite <- IHa1; simpl; omega).
+  destruct a2;
+    try (rewrite IHa1; rewrite IHa2; simpl; reflexivity);
+    destruct n;
+      try(rewrite IHa1; reflexivity);
+      try( rewrite <- IHa1; simpl; omega).
+  destruct a2;
+    try (rewrite IHa1; rewrite IHa2; simpl; reflexivity);
+    destruct n;
+      try(rewrite IHa1; reflexivity);
+      try( rewrite <- IHa1; simpl; omega).
 Qed.
 
 (*-- Check --*)
