sf/Assignment08_17.v
@@ -5,7 +5,29 @@ Require Export Assignment08_16.
 Lemma optimize_0plus_bexp_sound:
   btrans_sound optimize_0plus_bexp.
 Proof.
-  exact FILL_IN_HERE.
+  unfold btrans_sound. intros. induction b; simpl; try constructor.
+  - rename a into a1.
+    rename a0 into a2.
+    remember (optimize_0plus_aexp a1) as a1'.
+    remember (optimize_0plus_aexp a2) as a2'.
+    unfold bequiv. intros. simpl.
+    replace (aeval st a1) with (aeval st a1').
+    replace (aeval st a2) with (aeval st a2').
+    reflexivity.
+    rewrite Heqa2'. rewrite <- optimize_0plus_aexp_sound. reflexivity.
+    rewrite Heqa1'. rewrite <- optimize_0plus_aexp_sound. reflexivity.
+  - rename a into a1.
+    rename a0 into a2.
+    remember (optimize_0plus_aexp a1) as a1'.
+    remember (optimize_0plus_aexp a2) as a2'.
+    unfold bequiv. intros. simpl.
+    replace (aeval st a1) with (aeval st a1').
+    replace (aeval st a2) with (aeval st a2').
+    reflexivity.
+    rewrite Heqa2'. rewrite <- optimize_0plus_aexp_sound. reflexivity.
+    rewrite Heqa1'. rewrite <- optimize_0plus_aexp_sound. reflexivity.
+  - unfold bequiv. intros. simpl. rewrite IHb. reflexivity.
+  - unfold bequiv. intros. simpl. rewrite IHb1. rewrite IHb2. reflexivity.
 Qed.
 
 (*-- Check --*)
