sf/Assignment08_18.v
@@ -5,7 +5,25 @@ Require Export Assignment08_17.
 Lemma optimize_0plus_com_sound:
   ctrans_sound optimize_0plus_com.
 Proof.
-  exact FILL_IN_HERE.
+  unfold ctrans_sound. intros. induction c; simpl. apply refl_cequiv.
+  - unfold cequiv. intros. split. intros.
+    inversion H; subst. apply E_Ass. rewrite <- optimize_0plus_aexp_sound. reflexivity.
+    intros. inversion H; subst. apply E_Ass. rewrite <- optimize_0plus_aexp_sound. reflexivity.
+  - unfold cequiv. intros. split.
+    intros. inversion H; subst. apply E_Seq with st'0.
+      apply IHc1. apply H2.
+      apply IHc2. apply H5.
+    intros. inversion H; subst. apply E_Seq with st'0.
+      apply IHc1. apply H2.
+      apply IHc2. apply H5.
+  - unfold cequiv. intros. split.
+    intros. inversion H; subst.
+      apply E_IfTrue. rewrite <- optimize_0plus_bexp_sound. apply H5. apply IHc1. apply H6.
+      apply E_IfFalse. rewrite <- optimize_0plus_bexp_sound. apply H5. apply IHc2. apply H6.
+    intros. inversion H; subst.
+      apply E_IfTrue. rewrite <- optimize_0plus_bexp_sound in H5. apply H5. apply IHc1. apply H6.
+      apply E_IfFalse. rewrite <- optimize_0plus_bexp_sound in H5. apply H5. apply IHc2. apply H6.
+  - apply CWhile_congruence. apply optimize_0plus_bexp_sound. apply IHc.
 Qed.
 
 (*-- Check --*)
